rewrite formalization and some infrastructure (WIP)

doc/simple/coq/AlgoDef.v
@@ -9,56 +9,84 @@ Implicit Types x : var.
 Inductive AExpr : Set :=
   | AE_BVar : nat -> AExpr
   | AE_FVar : var -> AExpr
-  | AE_EVar : var -> AExpr
   | AE_Star : AExpr
   | AE_App : AExpr -> AExpr -> AExpr
   | AE_Lam : AExpr -> AExpr
-  | AE_Pi : AExpr -> AExpr -> AExpr
-  | AE_Let : AExpr -> AExpr -> AExpr
+  | AE_Pi : AType -> AType -> AExpr
   | AE_CastUp : AExpr -> AExpr
   | AE_CastDn : AExpr -> AExpr
-  | AE_Ann : AExpr -> AExpr -> AExpr.
-
-Inductive AType : Set :=
-  | AT_Forall : AType -> AType
+  | AE_Ann : AExpr -> AType -> AExpr
+  | AE_Forall: AType -> AExpr
+with
+AType : Set :=
+  | AT_TBVar : nat -> AType
+  | AT_TFVar : var -> AType
+  | AT_EVar : var -> AType
   | AT_Expr : AExpr -> AType.
 
 (** Open Operation *)
-
 
 Fixpoint AOpenRec (k : nat) (u : AExpr) (e : AExpr) {struct e} : AExpr :=
   match e with
   | AE_BVar i    => If k = i then u else (AE_BVar i)
   | AE_FVar x    => AE_FVar x
-  | AE_EVar x    => AE_EVar x
   | AE_Star      => AE_Star
   | AE_App e1 e2 => AE_App    (AOpenRec k u e1) (AOpenRec k u e2)
   | AE_Lam e     => AE_Lam   (AOpenRec (S k) u e)
-  | AE_Pi t1 t2  => AE_Pi     (AOpenRec k u t1) (AOpenRec (S k) u t2)
-  | AE_Let e1 e2 => AE_Let    (AOpenRec k u e1) (AOpenRec (S k) u e2)
+  | AE_Pi t1 t2  => AE_Pi     (AOpenTypRec k u t1) (AOpenTypRec (S k) u t2)
   | AE_CastUp e  => AE_CastUp (AOpenRec k u e)
   | AE_CastDn e  => AE_CastDn (AOpenRec k u e)
-  | AE_Ann e t   => AE_Ann    (AOpenRec k u e) (AOpenRec k u t)
+  | AE_Ann e t   => AE_Ann    (AOpenRec k u e) (AOpenTypRec k u t)
+  | AE_Forall s  => AE_Forall (AOpenTypRec (S k) u s)
+  end
+with
+AOpenTypRec (k : nat) (u : AExpr) (e : AType) {struct e} : AType :=
+  match e with
+  | AT_TBVar i   => AT_TBVar i
+  | AT_TFVar i   => AT_TFVar i
+  | AT_Expr t    => AT_Expr (AOpenRec k u t)
+  | AT_EVar i    => AT_EVar i
   end.
 
-Fixpoint AOpenTypRec (k : nat) (u : AExpr) (e : AType) {struct e} : AType :=
+Fixpoint ATOpenRec (k : nat) (u : AType) (e : AExpr) {struct e} : AExpr :=
   match e with
-  | AT_Forall s => AT_Forall (AOpenTypRec (S k) u s)
-  | AT_Expr t   => AT_Expr (AOpenRec k u t)
+  | AE_BVar i    => AE_BVar i
+  | AE_FVar x    => AE_FVar x
+  | AE_Star      => AE_Star
+  | AE_App e1 e2 => AE_App    (ATOpenRec k u e1) (ATOpenRec k u e2)
+  | AE_Lam e     => AE_Lam   (ATOpenRec (S k) u e)
+  | AE_Pi t1 t2  => AE_Pi     (ATOpenTypRec k u t1) (ATOpenTypRec (S k) u t2)
+  | AE_CastUp e  => AE_CastUp (ATOpenRec k u e)
+  | AE_CastDn e  => AE_CastDn (ATOpenRec k u e)
+  | AE_Ann e t   => AE_Ann    (ATOpenRec k u e) (ATOpenTypRec k u t)
+  | AE_Forall s  => AE_Forall (ATOpenTypRec (S k) u s)
+  end
+with
+ATOpenTypRec (k : nat) (u : AType) (e : AType) {struct e} : AType :=
+  match e with
+  | AT_TBVar i   => If i = k then u else (AT_TBVar i)
+  | AT_TFVar i   => AT_TFVar i
+  | AT_Expr t    => AT_Expr (ATOpenRec k u t)
+  | AT_EVar i    => AT_EVar i
   end.
 
 Definition AOpen e u := AOpenRec 0 u e.
 Definition AOpenT e u := AOpenTypRec 0 u e.
+Definition ATOpen e u := ATOpenRec 0 u e.
+Definition ATOpenT e u := ATOpenTypRec 0 u e.
 
-Notation "e @@ u" := (AOpen e u) (at level 67).
 Notation "e @ x" := (AOpen e (AE_FVar x)) (at level 67).
-Notation "e @@' u" := (AOpenT e u) (at level 67).
+Notation "e @@ u" := (AOpen e u) (at level 67).
+Notation "e @# x" := (ATOpen e (AT_TFVar x)) (at level 67).
+Notation "e @@# u" := (ATOpen e u) (at level 67).
 Notation "e @' x" := (AOpenT e (AE_FVar x)) (at level 67).
+Notation "e @@' u" := (AOpenT e u) (at level 67).
+Notation "e @#' x" := (ATOpenT e (AT_TFVar x)) (at level 67).
+Notation "e @@#' u" := (ATOpenT e u) (at level 67).
 
 (** Closed Terms *)
 Inductive ATerm : AExpr -> Prop :=
   | ATerm_Var : forall x, ATerm (AE_FVar x)
-  | ATerm_EVar : forall x, ATerm (AE_EVar x)
   | ATerm_Star : ATerm AE_Star
   | ATerm_App : forall e1 e2,
       ATerm e1 -> ATerm e2 -> ATerm (AE_App e1 e2)
@@ -66,31 +94,52 @@ Inductive ATerm : AExpr -> Prop :=
       (forall x, x \notin L -> ATerm (e @ x)) ->
       ATerm (AE_Lam e)
   | ATerm_Pi : forall L t1 t2,
-      ATerm t1 ->
-      (forall x, x \notin L -> ATerm (t2 @ x)) ->
+      ATermTy t1 ->
+      (forall x, x \notin L -> ATermTy (t2 @' x)) ->
       ATerm (AE_Pi t1 t2)
-  | ATerm_Let : forall L e1 e2,
-      ATerm e1 ->
-      (forall x, x \notin L -> ATerm (e2 @ x)) ->
-      ATerm (AE_Let e1 e2)
   | ATerm_CastUp : forall e,
       ATerm e -> ATerm (AE_CastUp e)
   | ATerm_CastDn : forall e,
       ATerm e -> ATerm (AE_CastDn e)
   | ATerm_Ann : forall t e,
-      ATerm t -> ATerm e -> ATerm (AE_Ann t e).
+      ATerm t -> ATermTy e -> ATerm (AE_Ann t e)
+  | ATerm_Forall : forall L t,
+      (forall x, x \notin L -> ATermTy (t @#' x))->
+      ATerm (AE_Forall t)
+with
+ATermTy : AType -> Prop :=
+  | ATermTy_TFVar : forall i, ATermTy (AT_TFVar i)
+  | ATermTy_EVar : forall x, ATermTy (AT_EVar x)
+  | ATermTy_Expr : forall e, ATerm e -> ATermTy (AT_Expr e)
+.
+
+Inductive AMono : AExpr -> Prop :=
+| DM_FVar : forall x, AMono (AE_FVar x)
+| DM_Star: AMono (AE_Star)
+| DM_App: forall e1 e2, AMono e1 -> AMono e2 -> AMono (AE_App e1 e2)
+| DM_Lam: forall L e, (forall x, x \notin L -> AMono (e @ x)) -> AMono (AE_Lam e)
+| DM_Pi: forall L s1 s2, ATMono s1 -> (forall x, x \notin L -> ATMono (s2 @' x)) -> AMono (AE_Pi s1 s2)
+| DM_CastUp: forall e, AMono e -> AMono (AE_CastUp e)
+| DM_CastDn: forall e, AMono e -> AMono (AE_CastDn e)
+| DM_Ann: forall e s, AMono e -> ATMono s -> AMono (AE_Ann e s)
+
+with
+ATMono: AType -> Prop :=
+| DM_TFVar : forall x, ATMono (AT_TFVar x)
+| DM_EVar : forall x, ATMono (AT_EVar x)
+| DM_Expr : forall e, AMono e -> ATMono (AT_Expr e).
 
 Definition ABody t :=
   exists L, forall x, x \notin L -> ATerm (t @ x).
 
-Inductive ATermTy : AType -> Prop :=
-  | ATermTy_Expr : forall e, ATerm e -> ATermTy (AT_Expr e)
-  | ATermTy_Forall : forall L t,
-      (forall x, x \notin L -> ATermTy (t @' x)) ->
-      ATermTy (AT_Forall t).
-
 Definition ABodyTy t :=
   exists L, forall x, x \notin L -> ATermTy (t @' x).
+
+Definition ATBody t :=
+  exists L, forall x, x \notin L -> ATerm (t @# x).
+
+Definition ATBodyTy t :=
+  exists L, forall x, x \notin L -> ATermTy (t @#' x).
 
 (** Substitution *)
 
@@ -98,21 +147,44 @@ Fixpoint ASubst (z : var) (u : AExpr) (e : AExpr) {struct e} : AExpr :=
   match e with
   | AE_BVar i    => AE_BVar i
   | AE_FVar x    => If x = z then u else (AE_FVar x)
-  | AE_EVar x    => If x = z then u else (AE_EVar x)
   | AE_Star      => AE_Star
   | AE_App e1 e2 => AE_App    (ASubst z u e1) (ASubst z u e2)
-  | AE_Lam e     => AE_Lam   (ASubst z u e)
-  | AE_Pi t1 t2  => AE_Pi     (ASubst z u t1) (ASubst z u t2)
-  | AE_Let e1 e2 => AE_Let    (ASubst z u e1) (ASubst z u e2)
+  | AE_Lam e     => AE_Lam    (ASubst z u e)
+  | AE_Pi t1 t2  => AE_Pi     (ATSubst z u t1) (ATSubst z u t2)
   | AE_CastUp e  => AE_CastUp (ASubst z u e)
   | AE_CastDn e  => AE_CastDn (ASubst z u e)
-  | AE_Ann e t   => AE_Ann    (ASubst z u e) (ASubst z u t)
+  | AE_Ann e t   => AE_Ann    (ASubst z u e) (ATSubst z u t)
+  | AE_Forall s  => AE_Forall (ATSubst z u s)
+  end
+with
+ATSubst (z : var) (u : AExpr) (e : AType) {struct e} : AType :=
+  match e with
+  | AT_Expr t    => AT_Expr (ASubst z u t)
+  | AT_TBVar x   => AT_TBVar x
+  | AT_TFVar x   => AT_TFVar x
+  | AT_EVar x    => AT_EVar x
   end.
 
-Fixpoint ATSubst (z : var) (u : AExpr) (e : AType) {struct e} : AType :=
+Fixpoint ASubstT (z : var) (u : AType) (e : AExpr) {struct e} : AExpr :=
   match e with
-  | AT_Forall s  => AT_Forall (ATSubst z u s)
-  | AT_Expr t    => AT_Expr (ASubst z u t)
+  | AE_BVar i    => AE_BVar i
+  | AE_FVar x    => AE_FVar x
+  | AE_Star      => AE_Star
+  | AE_App e1 e2 => AE_App    (ASubstT z u e1) (ASubstT z u e2)
+  | AE_Lam e     => AE_Lam    (ASubstT z u e)
+  | AE_Pi t1 t2  => AE_Pi     (ATSubstT z u t1) (ATSubstT z u t2)
+  | AE_CastUp e  => AE_CastUp (ASubstT z u e)
+  | AE_CastDn e  => AE_CastDn (ASubstT z u e)
+  | AE_Ann e t   => AE_Ann    (ASubstT z u e) (ATSubstT z u t)
+  | AE_Forall s  => AE_Forall (ATSubstT z u s)
+  end
+with
+ATSubstT (z : var) (u : AType) (e : AType) {struct e} : AType :=
+  match e with
+  | AT_TBVar i   => AT_TBVar i
+  | AT_TFVar i   => If i = z then u else (AT_TFVar i)
+  | AT_EVar i    => If i = z then u else (AT_EVar i)
+  | AT_Expr t    => AT_Expr (ASubstT z u t)
   end.
 
 (** Free Varialble *)
@@ -121,76 +193,35 @@ Fixpoint AFv (e : AExpr) {struct e} : vars :=
   match e with
   | AE_BVar i    => \{}
   | AE_FVar x    => \{x}
-  | AE_EVar x    => \{x}
   | AE_Star      => \{}
   | AE_App e1 e2 => (AFv e1) \u (AFv e2)
   | AE_Lam e     => AFv e
-  | AE_Pi t1 t2  => (AFv t1) \u (AFv t2)
-  | AE_Let e1 e2 => (AFv e1) \u (AFv e2)
+  | AE_Pi t1 t2  => (ATFv t1) \u (ATFv t2)
   | AE_CastUp e  => AFv e
   | AE_CastDn e  => AFv e
-  | AE_Ann e t   => (AFv e) \u (AFv t)
-  end.
-
-Fixpoint AFEv (e : AExpr) {struct e} : vars :=
+  | AE_Ann e t   => (AFv e) \u (ATFv t)
+  | AE_Forall  t => ATFv t
+  end
+with
+ATFv (e : AType) {struct e} : vars :=
   match e with
-  | AE_BVar i    => \{}
-  | AE_FVar x    => \{}
-  | AE_EVar x    => \{x}
-  | AE_Star      => \{}
-  | AE_App e1 e2 => (AFEv e1) \u (AFEv e2)
-  | AE_Lam e     => AFEv e
-  | AE_Pi t1 t2  => (AFEv t1) \u (AFEv t2)
-  | AE_Let e1 e2 => (AFEv e1) \u (AFEv e2)
-  | AE_CastUp e  => AFEv e
-  | AE_CastDn e  => AFEv e
-  | AE_Ann e t   => (AFEv e) \u (AFEv t)
-  end.
-
-Fixpoint ATFv (e : AType) {struct e} : vars :=
-  match e with
-  | AT_Forall s => ATFv s
-  | AT_Expr t   => AFv t
-  end.
-
-Fixpoint ATFEv (e : AType) {struct e} : vars :=
-  match e with
-  | AT_Forall s => ATFEv s
-  | AT_Expr t   => AFEv t
-  end.
+  | AT_TBVar x   => \{}
+  | AT_TFVar x   => \{x}
+  | AT_EVar x    => \{x}
+  | AT_Expr e    => AFv e
+  end
+  .
 
 (** Context *)
 
 Inductive ACtxT : Set :=
   | AC_Var : ACtxT
-  | AC_Typ : AExpr -> ACtxT
-  | AC_Bnd : AType -> AExpr -> ACtxT
+  | AC_Typ : AType -> ACtxT
+  | AC_TVar : ACtxT
   | AC_Unsolved_EVar : ACtxT
-  | AC_Solved_EVar : AExpr -> ACtxT.
+  | AC_Solved_EVar : AType -> ACtxT.
 
 Definition ACtx := LibEnv.env ACtxT.
-
-Fixpoint ACtxFv (G : ACtx) : vars :=
-  match G with
-  | nil => \{}
-  | cons (x, p) t =>
-    match p with
-    | AC_Typ ty => (AFv ty) \u (ACtxFv t)
-    | AC_Bnd s e => (ATFv s) \u (ACtxFv t)
-    | _ => ACtxFv t
-    end
-  end.
-
-Fixpoint ACtxFEv (G : ACtx) : vars :=
-  match G with
-  | nil => \{}
-  | cons (x, p) t =>
-    match p with
-    | AC_Typ ty => (AFEv ty) \u (ACtxFEv t)
-    | AC_Bnd s e => (ATFEv s) \u (ACtxFEv t)
-    | _ => ACtxFEv t
-    end
-  end.
 
 Definition ACtxSubst (G : ACtx) (e : AExpr) : AExpr :=
   LibList.fold_left
@@ -198,9 +229,9 @@ Definition ACtxSubst (G : ACtx) (e : AExpr) : AExpr :=
         match p with
         | AC_Var => v
         | AC_Typ _ => v
-        | AC_Bnd s t => ASubst x t v
+        | AC_TVar => v
         | AC_Unsolved_EVar => v
-        | AC_Solved_EVar t => ASubst x t v
+        | AC_Solved_EVar t => ASubstT x t v
         end) e G.
 
 Definition ACtxTSubst (G : ACtx) (e : AType) : AType :=
@@ -209,9 +240,9 @@ Definition ACtxTSubst (G : ACtx) (e : AType) : AType :=
         match p with
         | AC_Var => v
         | AC_Typ _ => v
-        | AC_Bnd s t => ATSubst x t v
+        | AC_TVar => v
         | AC_Unsolved_EVar => v
-        | AC_Solved_EVar t => ATSubst x t v
+        | AC_Solved_EVar t => ATSubstT x t v
         end) e G.
 
 Fixpoint ACtxUV (G : ACtx) {struct G} : ACtx :=
@@ -240,249 +271,244 @@ Inductive ARed : AExpr -> AExpr -> Prop :=
   | AR_CastDn : forall e e',
       ARed e e' -> ARed (AE_CastDn e) (AE_CastDn e')
   | AR_Ann : forall e t e',
-      ATerm t -> ARed e e' ->
+      ATermTy t -> ARed e e' ->
       ARed (AE_Ann e t) (AE_Ann e' t)
-  | AR_Let : forall e1 e2,
-      ATerm (AE_Let e1 e2) ->
-      ARed (AE_Let e1 e2) (e2 @@ e1).
-
-Inductive AGen : ACtx -> AExpr -> AType -> Prop :=
-  | AGen_Expr : forall G t,
-      ((AFEv t) \- (ACtxFEv G) = \{}) ->
-      AGen G t (AT_Expr (ACtxSubst G t))
-  | AGen_Poly : forall L G a t s,
-      a \in (AFEv t \- ACtxFEv G) ->
-     (forall x, x \notin L ->
-           AGen (G & x ~ AC_Typ AE_Star) (ASubst a (AE_FVar x) t) (s @@' (AE_FVar x))) ->
-      AGen G t (AT_Forall s).
-
-Inductive AInst : ACtx -> AType -> AExpr -> ACtx -> Prop :=
-  | AInst_Expr : forall G t,
-      AInst G (AT_Expr t) t G
-  | AInst_Poly : forall G H a s t,
-      a # G ->
-      AInst (G & a ~ AC_Unsolved_EVar) (s @@' (AE_EVar a)) t H ->
-      AInst G (AT_Forall s) t H.
+.
 
 Inductive AWTerm : ACtx -> AExpr -> Prop :=
   | AWTerm_Var : forall G x, binds x AC_Var G -> AWTerm G (AE_FVar x)
   | AWTerm_TypVar : forall G x t, binds x (AC_Typ t) G -> AWTerm G (AE_FVar x)
-  | AWTerm_LetVar : forall G x t e, binds x (AC_Bnd t e) G -> AWTerm G (AE_FVar x)
-  | AWTerm_EVar : forall G a, binds a AC_Unsolved_EVar G -> AWTerm G (AE_EVar a)
-  | AWTerm_Solved_EVar : forall G a t, binds a (AC_Solved_EVar t) G -> AWTerm G (AE_EVar a)
   | AWTerm_Star: forall G, AWTerm G AE_Star
   | AWTerm_App: forall e1 e2 G, AWTerm G e1 -> AWTerm G e2 -> AWTerm G (AE_App e1 e2)
   | AWTerm_Lam: forall e G L,
       (forall x, x \notin L -> AWTerm (G & x ~ AC_Var) (e @ x)) -> AWTerm G (AE_Lam e)
   | AWTerm_Pi: forall t1 t2 G L,
-      AWTerm G t1 ->
-      (forall x, x \notin L -> AWTerm (G & x ~ AC_Var) (t2 @ x)) -> AWTerm G (AE_Pi t1 t2)
-  | AWTerm_Let: forall e1 e2 G L,
-      AWTerm G e1 ->
-      (forall x, x \notin L -> AWTerm (G & x ~ AC_Var) (e2 @ x)) -> AWTerm G (AE_Let e1 e2)
+      AWTermT G t1 ->
+      (forall x, x \notin L -> AWTermT (G & x ~ AC_Var) (t2 @' x)) -> AWTerm G (AE_Pi t1 t2)
   | AWTerm_CastUp : forall e G, AWTerm G e -> AWTerm G (AE_CastUp e)
   | AWTerm_CastDn : forall e G, AWTerm G e -> AWTerm G (AE_CastDn e)
-  | AWTerm_Ann: forall e1 e2 G, AWTerm G e1 -> AWTerm G e2 -> AWTerm G (AE_Ann e1 e2)
-.
+  | AWTerm_Ann: forall e1 e2 G, AWTerm G e1 -> AWTermT G e2 -> AWTerm G (AE_Ann e1 e2)
+  | AWTerm_Forall: forall G L s,
+      (forall x, x \notin L -> AWTermT (G & x ~ AC_TVar) (s @#' x))
+      -> AWTerm G (AE_Forall s)
+with
+AWTermT : ACtx -> AType -> Prop :=
+  | AWTermT_TFVar: forall G i, binds i AC_TVar G -> AWTermT G (AT_TFVar i)
+  | AWTermT_Unsolved_EVar: forall G i, binds i AC_Unsolved_EVar G -> AWTermT G (AT_EVar i)
+  | AWTermT_Solved_EVar: forall G i t, binds i (AC_Solved_EVar t) G -> AWTermT G (AT_EVar i)
+  | AWTermT_Expr: forall G e, AWTerm G e -> AWTermT G (AT_Expr e).
 
-Inductive AWTermT : ACtx -> AType -> Prop :=
-  | AWTermT_Forall : forall G s L,
-      (forall x, x \notin L -> AWTermT (G & x ~ AC_Typ AE_Star) (s @' x)) -> AWTermT G (AT_Forall s)
-  | AWTermT_Expr: forall G e,
-      AWTerm G e -> AWTermT G (AT_Expr e).
-
-Inductive AResolveEVar : ACtx -> var -> AExpr -> AExpr -> ACtx -> Prop :=
+Inductive AResolveEVar : ACtx -> var -> AType -> AType -> ACtx -> Prop :=
   | AResolveEVar_EVar_Before : forall a b G1 G2 G3,
-      AResolveEVar (G1 & b ~ AC_Unsolved_EVar & G2 & a ~ AC_Unsolved_EVar & G3) a (AE_EVar b) (AE_EVar b)
+      AResolveEVar (G1 & b ~ AC_Unsolved_EVar & G2 & a ~ AC_Unsolved_EVar & G3) a (AT_EVar b) (AT_EVar b)
                    (G1 & b ~ AC_Unsolved_EVar & G2 & a ~ AC_Unsolved_EVar & G3)
   | AResolveEVar_EVar_After : forall a b G1 G2 G3 a1,
-      AResolveEVar (G1 & a ~ AC_Unsolved_EVar & G2 & b ~ AC_Unsolved_EVar & G3) a (AE_EVar b) (AE_EVar a1)
-                   (G1 & a1 ~ AC_Unsolved_EVar & a ~ AC_Unsolved_EVar & G2 & b ~ AC_Solved_EVar (AE_EVar a1) & G3)
+      AResolveEVar (G1 & a ~ AC_Unsolved_EVar & G2 & b ~ AC_Unsolved_EVar & G3) a (AT_EVar b) (AT_EVar a1)
+                   (G1 & a1 ~ AC_Unsolved_EVar & a ~ AC_Unsolved_EVar & G2 & b ~ AC_Solved_EVar (AT_EVar a1) & G3)
   | AResolveEVar_Pi : forall a t1 t2 t3 t4 G H1 H L,
       AResolveEVar G a t1 t3 H1 ->
-      (forall x, x \notin L -> AResolveEVar H1 a (ACtxSubst H1 (t2 @ x)) (ACtxSubst H1 (t4 @ x)) H) ->
-      AResolveEVar G a (AE_Pi t1 t2) (AE_Pi t3 t4) H
-  | AResolveEVar_Var : forall a x G, AResolveEVar G a (AE_FVar x) (AE_FVar x) G
-  | AResolveEVar_Star : forall a G, AResolveEVar G a AE_Star AE_Star G
-  | AResolveEVar_App : forall a t1 t2 G, AResolveEVar G a (AE_App t1 t2) (AE_App t1 t2) G
-  | AResolveEVar_Lam : forall a t1 G, AResolveEVar G a (AE_Lam t1) (AE_Lam t1) G
-  | AResolveEVar_Let : forall a t1 t2 G, AResolveEVar G a (AE_Let t1 t2) (AE_Let t1 t2) G
-  | AResolveEVar_CastUp : forall a t G, AResolveEVar G a (AE_CastUp t) (AE_CastUp t) G
-  | AResolveEVar_CastDn : forall a t G, AResolveEVar G a (AE_CastDn t) (AE_CastDn t) G
-  | AResolveEVar_Ann : forall a t1 t2 G, AResolveEVar G a (AE_Ann t1 t2) (AE_Ann t1 t2) G
+      (forall x, x \notin L -> AResolveEVar H1 a (ACtxTSubst H1 (t2 @' x)) (ACtxTSubst H1 (t4 @' x)) H) ->
+      AResolveEVar G a (AT_Expr (AE_Pi t1 t2)) (AT_Expr (AE_Pi t3 t4)) H
+  | AResolveEVar_Var : forall a x G, AResolveEVar G a (AT_Expr (AE_FVar x)) (AT_Expr (AE_FVar x)) G
+  | AResolveEVar_TBVar : forall (x:nat) a G, AResolveEVar G a (AT_TBVar x) (AT_TBVar x) G
+  | AResolveEVar_TFVar : forall a x G, AResolveEVar G a (AT_TFVar x) (AT_TFVar x) G
+  | AResolveEVar_Star : forall a G, AResolveEVar G a (AT_Expr AE_Star) (AT_Expr AE_Star) G
+  | AResolveEVar_App : forall a t1 t2 G, AResolveEVar G a (AT_Expr (AE_App t1 t2)) (AT_Expr (AE_App t1 t2)) G
+  | AResolveEVar_Lam : forall a t1 G, AResolveEVar G a (AT_Expr (AE_Lam t1)) (AT_Expr (AE_Lam t1)) G
+  | AResolveEVar_CastUp : forall a t G, AResolveEVar G a (AT_Expr (AE_CastUp t)) (AT_Expr (AE_CastUp t)) G
+  | AResolveEVar_CastDn : forall a t G, AResolveEVar G a (AT_Expr (AE_CastDn t)) (AT_Expr (AE_CastDn t)) G
+  | AResolveEVar_Ann : forall a t1 t2 G, AResolveEVar G a (AT_Expr (AE_Ann t1 t2)) (AT_Expr (AE_Ann t1 t2)) G
 .
 
-Inductive AUnify : ACtx -> AExpr -> AExpr -> ACtx -> Prop :=
-  | AUnify_Var : forall x G, binds x AC_Var G -> AUnify G (AE_FVar x) (AE_FVar x) G
-  | AUnify_Typed_Var : forall x G t, binds x (AC_Typ t) G -> AUnify G (AE_FVar x) (AE_FVar x) G
-  | AUnify_Bnd_Var : forall x t s G, binds x (AC_Bnd s t) G -> AUnify G (AE_FVar x) (AE_FVar x) G
-  | AUnify_EVar : forall a G, binds a AC_Unsolved_EVar G -> AUnify G (AE_EVar a) (AE_EVar a) G
+Inductive ARFMode := Plus | Minus.
+
+Inductive AResolveForall : ACtx -> var -> ARFMode -> AType -> AType -> ACtx -> Prop :=
+  | AResolveForall_Poly: forall a L G1 G2 H s t,
+      (forall a1, a1 \notin L ->
+             AResolveForall (G1 & a1 ~ AC_Unsolved_EVar & a ~ AC_Unsolved_EVar & G2)
+                            a Plus (s @@#' (AT_EVar a1)) t H) ->
+      AResolveForall (G1 & a ~ AC_Unsolved_EVar & G2) a Plus (AT_Expr (AE_Forall s)) t H
+  | AResolveForall_Pi1: forall G s1 s2 t1 t2 H1 H a,
+      AResolveForall G a Plus s1 t1 H1 ->
+      AResolveForall H1 a Minus s2 t2 H ->
+      AResolveForall G a Minus (AT_Expr (AE_Pi s1 s2)) (AT_Expr (AE_Pi t1 t2)) H
+  | AResolveForall_Pi2: forall G s1 s2 t1 t2 H1 H a,
+      AResolveForall G a Minus s1 t1 H1 ->
+      AResolveForall H1 a Plus s2 t2 H ->
+      AResolveForall G a Plus (AT_Expr (AE_Pi s1 s2)) (AT_Expr (AE_Pi t1 t2)) H
+  | AResolveForall_Mono : forall G H a m t,
+      ATMono t -> AResolveForall G a m t t H.
+
+Inductive AUnify : ACtx -> AType -> AType -> ACtx -> Prop :=
+  | AUnify_Var : forall x G, binds x AC_Var G -> AUnify G (AT_Expr (AE_FVar x)) (AT_Expr (AE_FVar x)) G
+  | AUnify_Typed_Var : forall x G t, binds x (AC_Typ t) G -> AUnify G (AT_Expr (AE_FVar x)) (AT_Expr (AE_FVar x)) G
+  | AUnify_EVar : forall a G, binds a AC_Unsolved_EVar G -> AUnify G (AT_EVar a) (AT_EVar a) G
+  | AUnify_TVar : forall a G, binds a AC_TVar G -> AUnify G (AT_TFVar a) (AT_TFVar a) G
   (* no case for solved evar since it is fully applied under context *)
-  | AUnify_Star : forall G, AUnify G (AE_Star) (AE_Star) G
+  | AUnify_Star : forall G, AUnify G (AT_Expr (AE_Star)) (AT_Expr (AE_Star)) G
   | AUnify_App : forall t1 t2 t3 t4 G H1 H,
-      AUnify G t1 t2 H1 ->
-      AUnify H1 (ACtxSubst H1 t3) (ACtxSubst H1 t4) H ->
-      AUnify G (AE_App t1 t3) (AE_App t2 t3) H
-  | AUnify_Let : forall t1 t2 t3 t4 G H1 H L,
-      AUnify G t1 t2 H1 ->
-      (forall x, x \notin L -> AUnify (H1 & x ~ AC_Var) (ACtxSubst H1 (t3 @ x)) (ACtxSubst H1 (t4 @ x)) (H & x ~ AC_Var)) ->
-      AUnify G (AE_Let t1 t3) (AE_Let t2 t4) H
+      AUnify G (AT_Expr t1) (AT_Expr t2) H1 ->
+      AUnify H1 (AT_Expr (ACtxSubst H1 t3)) (AT_Expr (ACtxSubst H1 t4)) H ->
+      AUnify G (AT_Expr (AE_App t1 t3)) (AT_Expr (AE_App t2 t3)) H
   | AUnify_Lam : forall t1 t2 G H L,
-      (forall x, x \notin L -> AUnify (G & x ~ AC_Var) (t1 @ x) (t2 @ x) (H & x ~ AC_Var)) ->
-      AUnify G (AE_Lam t1) (AE_Lam t2) H
+      (forall x, x \notin L -> AUnify (G & x ~ AC_Var) (AT_Expr (t1 @ x)) (AT_Expr (t2 @ x)) (H & x ~ AC_Var)) ->
+      AUnify G (AT_Expr (AE_Lam t1)) (AT_Expr (AE_Lam t2)) H
   | AUnify_CastUp : forall t1 t2 G H,
-      AUnify G t1 t2 H ->
-      AUnify G (AE_CastUp t1) (AE_CastUp t2) H
+      AUnify G (AT_Expr t1) (AT_Expr t2) H ->
+      AUnify G (AT_Expr (AE_CastUp t1)) (AT_Expr (AE_CastUp t2)) H
   | AUnify_CastDn : forall t1 t2 G H,
-      AUnify G t1 t2 H ->
-      AUnify G (AE_CastDn t1) (AE_CastDn t2) H
+      AUnify G (AT_Expr t1) (AT_Expr t2) H ->
+      AUnify G (AT_Expr (AE_CastDn t1)) (AT_Expr (AE_CastDn t2)) H
   | AUnify_Pi : forall t1 t2 t3 t4 G H1 H L,
       AUnify G t1 t3 H1 ->
-      (forall x, x \notin L -> AUnify (H1 & x ~ AC_Typ t1) (ACtxSubst H1 (t2 @ x)) (ACtxSubst H1 (t4 @ x)) (H & x ~ AC_Typ t1)) ->
-      AUnify G (AE_Pi t1 t2) (AE_Pi t3 t4) H
+      (forall x, x \notin L -> AUnify (H1 & x ~ AC_Typ t1) (ACtxTSubst H1 (t2 @' x)) (ACtxTSubst H1 (t4 @' x)) (H & x ~ AC_Typ t1)) ->
+      AUnify G (AT_Expr (AE_Pi t1 t2)) (AT_Expr (AE_Pi t3 t4)) H
   | AUnify_Ann : forall t1 t2 t3 t4 G H1 H,
-      AUnify G t1 t2 H1 ->
-      AUnify H1 (ACtxSubst H1 t3) (ACtxSubst H1 t4) H ->
-      AUnify G (AE_Ann t1 t3) (AE_Ann t2 t3) H
+      AUnify G (AT_Expr t1) (AT_Expr t2) H1 ->
+      AUnify H1 (ACtxTSubst H1 t3) (ACtxTSubst H1 t4) H ->
+      AUnify G (AT_Expr (AE_Ann t1 t3)) (AT_Expr (AE_Ann t2 t3)) H
   | AUnify_EVarTy : forall a t1 t2 G H1 H2,
-      a \notin (AFv (t1)) ->
+      a \notin ATFv (t1) ->
       AResolveEVar G a t1 t2 (H1 & a ~ AC_Unsolved_EVar & H2) ->
-      AWTerm H1 t2 ->
-      AUnify G (AE_EVar a) t1 (H1 & a ~ AC_Solved_EVar t2 & H2)
+      AWTermT H1 t2 ->
+      AUnify G (AT_EVar a) t1 (H1 & a ~ AC_Solved_EVar t2 & H2)
   | AUnify_TyEVar : forall a t1 t2 G H1 H2,
-      a \notin (AFv (t1)) ->
+      a \notin ATFv (t1) ->
       AResolveEVar G a t1 t2 (H1 & a ~ AC_Unsolved_EVar & H2) ->
-      AWTerm H1 t2 ->
-      AUnify G t1 (AE_EVar a) (H1 & a ~ AC_Solved_EVar t2 & H2).
+      AWTermT H1 t2 ->
+      AUnify G t1 (AT_EVar a) (H1 & a ~ AC_Solved_EVar t2 & H2).
 
-Inductive AMode := Inf | Chk | App.
+Inductive AMode := Inf | Chk | App : AType -> AMode.
 
-Inductive ATyping : AMode -> ACtx -> AExpr -> AExpr -> ACtx -> Prop :=
-  | ATI_Ax : forall G, AWf G -> ATyping Inf G AE_Star AE_Star G
+Inductive ASubtyping : ACtx -> AType -> AType -> ACtx -> Prop :=
+  | ASub_PolyR: forall G v s1 s2 H I,
+      v # G ->
+      ASubtyping (G & v ~ AC_TVar) s1 (s2 @#' v) (H & v ~ AC_TVar & I) ->
+      ASubtyping G s1 (AT_Expr (AE_Forall s2)) H
+  | ASub_PolyL: forall G s1 s2 H a,
+      a # G ->
+      ASubtyping (G & a ~ AC_Unsolved_EVar) (s1 @@#' (AT_EVar a)) s2 H ->
+      ASubtyping G (AT_Expr (AE_Forall s1)) s2 H
+  | ASub_Pi: forall G s1 s2 s3 s4 H I x H1,
+      ASubtyping G s3 s1 H1 ->
+      ASubtyping (H1 & x ~ AC_Typ s1) (ACtxTSubst H1 (s2 @' x)) (ACtxTSubst H1 (s4 @' x)) (H & x ~ AC_Typ s1 & I) ->
+      ASubtyping G (AT_Expr (AE_Pi s1 s2)) (AT_Expr (AE_Pi s3 s4)) H
+  | ASub_EVarL: forall a s G1 G2 H1 H t,
+      AResolveForall (G1 & a ~ AC_Unsolved_EVar & G2) a Minus s t H1 ->
+      AUnify H1 (AT_EVar a) t H ->
+      ASubtyping (G1 & a ~ AC_Unsolved_EVar & G2) (AT_EVar a) s H
+  | ASub_EVarR: forall a s G1 G2 H1 H t,
+      AResolveForall (G1 & a ~ AC_Unsolved_EVar & G2) a Plus s t H1 ->
+      AUnify H1 (AT_EVar a) t H ->
+      ASubtyping (G1 & a ~ AC_Unsolved_EVar & G2) s (AT_EVar a) H
+  | ASub_Unify: forall G H s1 s2,
+      AUnify G s1 s2 H ->
+      ASubtyping G s1 s2 H.
+
+Inductive ATyping : AMode -> ACtx -> AType -> AType -> ACtx -> Prop :=
+  | ATI_Ax : forall G, AWf G -> ATyping Inf G (AT_Expr AE_Star) (AT_Expr AE_Star) G
   | ATI_Var : forall G x t, AWf G -> binds x (AC_Typ t) G ->
-                            ATyping Inf G (AE_FVar x) t G
+                       ATyping Inf G (AT_Expr (AE_FVar x)) t G
   | ATI_EVar : forall G x, AWf G -> binds x AC_Unsolved_EVar G ->
-                            ATyping Inf G (AE_EVar x) AE_Star G
+                      ATyping Inf G (AT_EVar x) (AT_Expr AE_Star) G
   | ATI_Solved_EVar : forall G x t, AWf G -> binds x (AC_Solved_EVar t) G ->
-                            ATyping Inf G (AE_EVar x) AE_Star G
-  | ATI_LetVar : forall G H x s t t2,
-      AWf G -> binds x (AC_Bnd s t) G ->
-      AInst G s t2 H ->
-      ATyping Inf G (AE_FVar x) t2 H
+                               ATyping Inf G (AT_EVar x) (AT_Expr AE_Star) G
+  | ATI_TVar : forall G x, AWf G -> binds x AC_TVar G ->
+                      ATyping Inf G (AT_TFVar x) (AT_Expr AE_Star) G
   | ATI_Ann : forall G H H1 e t,
-      AWTerm G (AE_Ann e t) ->
-      ATyping Chk G t AE_Star H1 ->
-      ATyping Chk H1 e t H ->
-      ATyping Inf G (AE_Ann e t) t H
+      AWTermT G (AT_Expr (AE_Ann e t)) ->
+      ATyping Chk G t (AT_Expr AE_Star) H1 ->
+      ATyping Chk H1 (AT_Expr e) t H ->
+      ATyping Inf G (AT_Expr (AE_Ann e t)) t H
   | ATI_Pi : forall G H1 H I t1 t2 x,
-      AWTerm G (AE_Pi t1 t2) ->
+      AWTermT G (AT_Expr (AE_Pi t1 t2)) ->
+      ATyping Chk G t1 (AT_Expr AE_Star) H1 ->
       x # G ->
-      ATyping Chk G t1 AE_Star H1 ->
-      ATyping Chk (H1 & (x ~ AC_Typ t1)) (t2 @ x) AE_Star
-                  (H & (x ~ AC_Typ t1) & I) ->
-      ATyping Inf G (AE_Pi t1 t2) AE_Star H
+      ATyping Chk (H1 & x ~ AC_Typ t1) (t2 @' x) (AT_Expr AE_Star)
+                  (H & x ~ AC_Typ t1 & I) ->
+      ATyping Inf G (AT_Expr (AE_Pi t1 t2)) (AT_Expr AE_Star) H
   | ATI_Lam : forall G H I e a t2 x,
-      AWTerm G (AE_Lam e) ->
+      AWTermT G (AT_Expr (AE_Lam e)) ->
       x # G ->
       a # G ->
-      ATyping Inf (G & a ~ AC_Unsolved_EVar & x ~ AC_Typ (AE_EVar a))
-                  (e @ x) (t2 @ x)
-                  (H & x ~ AC_Typ (AE_EVar a) & I) ->
-      ATyping Inf G (AE_Lam e) (AE_Pi (AE_EVar a) (ACtxSubst I t2)) (H & ACtxUV I)
-  | ATI_App : forall G H1 H e1 e2 t1 t2,
-      AWTerm G (AE_App e1 e2) ->
-      ATyping Inf G e1 (AE_Pi t1 t2) H1 ->
-      ATyping App H1 (AE_App (ACtxSubst H1 t1) e2) t2 H ->
-      ATyping Inf G (AE_App e1 e2) t2 H
-  | ATI_Let : forall G H1 H I e1 e2 s t1 t2 x,
-      AWTerm G (AE_Let e1 e2) ->
-      x # G -> x \notin AFv t2 ->
-      ATyping Inf G e1 t1 H1 ->
-      AGen H1 t1 s ->
-      ATyping Inf (H1 & x ~ AC_Bnd s e1) (e2 @ x) (t2 @ x)
-                  (H & x ~ AC_Bnd s e1 & I) ->
-      ATyping Inf G (AE_Let e1 e2) (ACtxSubst I (t2 @@ e1)) (H & ACtxUV I)
+      ATyping Inf (G & a ~ AC_Unsolved_EVar & x ~ AC_Typ (AT_EVar a))
+                  (AT_Expr (e @ x)) (t2 @' x)
+                  (H & x ~ AC_Typ (AT_EVar a) & I) ->
+      ATyping Inf G (AT_Expr (AE_Lam e)) (AT_Expr (AE_Pi (AT_EVar a) (ACtxTSubst I t2))) (H & ACtxUV I)
+  | ATI_App : forall G H1 H e1 e2 s1 s2,
+      AWTermT G (AT_Expr (AE_App e1 e2)) ->
+      ATyping Inf G (AT_Expr e1) s1 H1 ->
+      ATyping (App (ACtxTSubst H1 s1)) H1 (AT_Expr e2) s2 H ->
+      ATyping Inf G (AT_Expr (AE_App e1 e2)) s2 H
   | ATI_CastDn : forall G H e t1 t2,
-      AWTerm G (AE_CastDn e) ->
-      ATyping Inf G e t1 H ->
+      AWTermT G (AT_Expr (AE_CastDn e)) ->
+      ATyping Inf G (AT_Expr e) (AT_Expr t1) H ->
       ARed (ACtxSubst H t1) t2 ->
-      ATyping Inf G (AE_CastDn e) t2 H
+      ATyping Inf G (AT_Expr (AE_CastDn e)) (AT_Expr t2) H
+  | ATI_Forall: forall G s H a I,
+      AWTermT G (AT_Expr (AE_Forall s)) ->
+      a # G ->
+      ATyping Chk (G & a ~ AC_TVar) (s @#' a) (AT_Expr AE_Star) (H & a ~ AC_TVar & I) ->
+      ATyping Inf G (AT_Expr (AE_Forall s)) (AT_Expr AE_Star) H
 
-  | ATC_Lam : forall G H I e t1 t2 x,
-      AWTerm G (AE_Lam e) -> AWTerm G (AE_Pi t1 t2) ->
+  | ATC_Lam : forall G H I e s1 s2 x,
+      AWTermT G (AT_Expr (AE_Lam e)) ->
       x # G ->
-      ATyping Chk (G & x ~ AC_Typ t1) (e @ x) (t2 @ x)
-                  (H & x ~ AC_Typ t1 & I) ->
-      ATyping Chk G (AE_Lam e) (AE_Pi t1 t2) H
-  | ATC_Let : forall G H1 H I e1 e2 s t1 t2 x,
-      AWTerm G (AE_Let e1 e2) -> AWTerm G t2 ->
-      x # G -> x \notin AFv t2 ->
-      ATyping Inf G e1 t1 H1 ->
-      AGen H1 t1 s ->
-      ATyping Chk (H1 & x ~ (AC_Bnd s e1)) (e2 @ x) (t2 @ x)
-                  (H & x ~ AC_Bnd s e1 & I) ->
-      ATyping Chk G (AE_Let e1 e2) (ACtxSubst I (t2 @@ e1)) (H & ACtxUV I)
+      ATyping Chk (G & x ~ AC_Typ s1) (AT_Expr (e @ x)) (s2 @' x)
+                  (H & x ~ AC_Typ s1 & I) ->
+      ATyping Chk G (AT_Expr (AE_Lam e)) (AT_Expr (AE_Pi s1 s2)) H
   | ATC_CastUp : forall G H e t1 t2,
-      AWTerm G (AE_CastUp e) -> AWTerm G t2 ->
+      AWTermT G (AT_Expr (AE_CastUp e)) ->
       ARed (ACtxSubst G t2) t1 ->
-      ATyping Chk G e t1 H ->
-      ATyping Chk G (AE_CastUp e) t2 H
-  | ATC_Sub : forall G H1 H e t1 t2,
-      AWTerm G e -> AWTerm G t2 ->
-      ATyping Inf G e t1 H1 ->
-      AUnify H1 (ACtxSubst H1 t1) (ACtxSubst H1 t2) H ->
-      ATyping Chk G e t2 H
+      ATyping Chk G (AT_Expr e) (AT_Expr t1) H ->
+      ATyping Chk G (AT_Expr (AE_CastUp e)) (AT_Expr t2) H
+  | ATC_Sub : forall G H1 H e s1 s2,
+      ATyping Inf G e s1 H1 ->
+      ASubtyping H1 (ACtxTSubst H1 s1) (ACtxTSubst H1 s2) H ->
+      ATyping Chk G e s2 H
 
-  | ATA_Pi : forall G H e t1 t2 m H1,
-      AWTerm G (AE_App (AE_Pi t1 t2) e) ->
-      ATyping m G (AE_Pi t1 t2) AE_Star H1 ->
-      ATyping Chk G e t1 H ->
-      ATyping App G (AE_App (AE_Pi t1 t2) e) (t2 @@ e) H
+  | ATA_Pi : forall G H e s1 s2,
+      ATyping Chk G (AT_Expr e) s1 H ->
+      ATyping (App (AT_Expr (AE_Pi s1 s2))) G (AT_Expr e) (s2 @@' e) H
   | ATA_EVar : forall G1 G2 H a e a1 a2,
-      AWTerm (G1 & a ~ AC_Unsolved_EVar & G2) (AE_App (AE_EVar a) e) ->
       AWf (G1 & a ~ AC_Unsolved_EVar & G2) ->
+      AWTermT (G1 & a ~ AC_Unsolved_EVar & G2) (AT_Expr e) ->
       ATyping Chk (G1 & a2 ~ AC_Unsolved_EVar & a1 ~ AC_Unsolved_EVar &
-                    a ~ AC_Solved_EVar (AE_Pi (AE_EVar a1) (AE_EVar a2)) & G2)
-                  e (AE_EVar a1) H ->
-      ATyping App (G1 & a ~ AC_Unsolved_EVar & G2) (AE_App (AE_EVar a) e) (AE_EVar a2) H
+                    a ~ AC_Solved_EVar (AT_Expr (AE_Pi (AT_EVar a1) (AT_EVar a2))) & G2)
+                  (AT_Expr e) (AT_EVar a1) H ->
+      ATyping (App (AT_EVar a)) (G1 & a ~ AC_Unsolved_EVar & G2) (AT_Expr e) (AT_EVar a2) H
+  | ATA_Forall : forall G s e s2 H a,
+      AWTermT G e ->
+      a # G ->
+      ATyping (App (s @@#' (AT_EVar a))) (G & a ~ AC_Unsolved_EVar) e s2 H ->
+      ATyping (App (AT_Expr (AE_Forall s))) G e s2 H
 
 with AWfTyp : ACtx -> AType -> Prop :=
-     | AWf_Poly : forall L G s,
-         (forall x, x \notin L -> AWfTyp (G & x ~ AC_Typ AE_Star) (s @' x)) ->
-         AWfTyp G (AT_Forall s)
-     | AWf_Expr : forall G H t,
-         ATyping Chk G t AE_Star (G & H) ->
-         AWfTyp G (AT_Expr t)
+     | AWf_Expr : forall G H s,
+         ATyping Chk G s (AT_Expr AE_Star) (G & H) ->
+         AWfTyp G s
 
 with AWf : ACtx -> Prop :=
      | AWf_Nil : AWf empty
      | AWf_Var : forall G x,
          AWf G -> x # G ->
          AWf (G & x ~ AC_Var)
-     | AWf_TyVar : forall G x t,
-         AWf G -> x # G ->
-         AWfTyp G (AT_Expr t) ->
-         AWf (G & x ~ AC_Typ t)
-     | AWf_LetVar : forall G H x s t,
-         AWf G -> x # G ->
-         AWfTyp G (AT_Expr s) ->
-         ATyping Chk G t (ACtxSubst G s) (G & H) ->
-         AWf (G & x ~ AC_Bnd (AT_Expr s) t)
-     | AWf_LetVar2 : forall L G x s t,
+     | AWf_TVar : forall G a,
+         AWf G -> a # G ->
+         AWf (G & a ~ AC_TVar)
+     | AWf_TyVar : forall G x s,
          AWf G -> x # G ->
          AWfTyp G s ->
-         (forall y, y \notin L ->
-                 AWf (G & y ~ AC_Typ AE_Star & x ~ AC_Bnd (AOpenT s (AE_FVar y)) t)) ->
-         AWf (G & x ~ AC_Bnd (AT_Forall s) t)
+         AWf (G & x ~ AC_Typ s)
      | AWf_Ctx_Unsolved_EVar : forall G x,
          AWf G -> x # G ->
          AWf (G & x ~ AC_Unsolved_EVar)
      | AWf_Ctx_Solved_EVar : forall G x t,
          AWf G -> x # G ->
-         AWfTyp G (AT_Expr t) ->
+         ATMono t ->
+         AWfTyp G t ->
          AWf (G & x ~ AC_Solved_EVar t)
 .
 
 Definition ATypingI := ATyping Inf.
 Definition ATypingC := ATyping Chk.
-Definition ATypingApp := ATyping App.
