doc/simple/coq/AlgoInfra.v
@@ -27,8 +27,8 @@ Scheme atyping_induct := Induction for ATyping Sort Prop
   with awftyp_induct := Induction for AWfTyp Sort Prop
   with awf_induct := Induction for AWf Sort Prop.
 
-Hint Constructors ARed ATyping AMode AWfTyp AWf AInst AGen
-     AUnify AResolveEVar AWTerm.
+Hint Constructors ARed ATyping AMode ARFMode AWfTyp AWf
+     AUnify AResolveEVar AResolveForall AWTerm AWTermT.
 
 (** Substitution *)
 
@@ -37,78 +37,135 @@ Hint Constructors ATerm.
 (* Substitution on indices is identity on well-formed terms. *)
 
 Lemma aopen_rec_term_core :forall e j v i u, i <> j ->
-  AOpenRec j v e = AOpenRec i u (AOpenRec j v e) -> e = AOpenRec i u e.
+  AOpenRec j v e = AOpenRec i u (AOpenRec j v e) -> e = AOpenRec i u e
+with
+aopent_rec_term_core :forall e j v i u, i <> j ->
+  AOpenTypRec j v e = AOpenTypRec i u (AOpenTypRec j v e) -> e = AOpenTypRec i u e.
 Proof.
   induction e; introv Neq Equ;
   simpl in *; inversion* Equ; f_equal*.  
   case_nat*. case_nat*.
+Proof.
+  induction e; introv Neq Equ;
+  simpl in *; inversion* Equ; f_equal*.
 Qed.
 
 Lemma atopen_rec_term_core :forall e j v i u, i <> j ->
-  AOpenTypRec j v e = AOpenTypRec i u (AOpenTypRec j v e) -> e = AOpenTypRec i u e.
+  ATOpenRec j v e = ATOpenRec i u (ATOpenRec j v e) -> e = ATOpenRec i u e
+with
+atopent_rec_term_core :forall e j v i u, i <> j ->
+  ATOpenTypRec j v e = ATOpenTypRec i u (ATOpenTypRec j v e) -> e = ATOpenTypRec i u e.
 Proof.
   induction e; introv Neq Equ;
-    simpl in *; inversion* Equ; f_equal*.
-  apply aopen_rec_term_core with (j := j) (v := v).
-  auto. auto.
+  simpl in *; inversion* Equ; f_equal*.
+Proof.
+  induction e; introv Neq Equ;
+  simpl in *; inversion* Equ; f_equal*.
+  case_nat*. case_nat*.
+Qed.
+
+Lemma aopen_atopen_rec_term_core :forall e j v i u, i <> j ->
+  ATOpenRec j v e = AOpenRec i u (ATOpenRec j v e) -> e = AOpenRec i u e
+with
+aopent_atopent_rec_term_core :forall e j v i u, i <> j ->
+  ATOpenTypRec j v e = AOpenTypRec i u (ATOpenTypRec j v e) -> e = AOpenTypRec i u e.
+Proof.
+  induction e; introv Neq Equ;
+  simpl in *; inversion* Equ; f_equal*.
+Proof.
+  induction e; introv Neq Equ;
+  simpl in *; inversion* Equ; f_equal*.
+Qed.
+
+Lemma atopen_aopen_rec_term_core :forall e j v i u, i <> j ->
+  AOpenRec j v e = ATOpenRec i u (AOpenRec j v e) -> e = ATOpenRec i u e
+with
+atopent_aopent_rec_term_core :forall e j v i u, i <> j ->
+  AOpenTypRec j v e = ATOpenTypRec i u (AOpenTypRec j v e) -> e = ATOpenTypRec i u e.
+Proof.
+  induction e; introv Neq Equ;
+  simpl in *; inversion* Equ; f_equal*.
+Proof.
+  induction e; introv Neq Equ;
+  simpl in *; inversion* Equ; f_equal*.
 Qed.
 
 Lemma aopen_rec_term : forall t u,
-  ATerm t -> forall k, t = AOpenRec k u t.
+  ATerm t -> forall k, t = AOpenRec k u t
+with aopent_rec_term : forall t u,
+  ATermTy t -> forall k, t = AOpenTypRec k u t.
 Proof.
   induction 1; intros; simpl; f_equal*.
   unfolds AOpen. pick_fresh x.
    apply* (@aopen_rec_term_core e 0 (AE_FVar x)).
   unfolds AOpen. pick_fresh x.
-   apply* (@aopen_rec_term_core t2 0 (AE_FVar x)).
+   apply* (@aopent_rec_term_core t2 0 (AE_FVar x)).
   unfolds AOpen. pick_fresh x.
-   apply* (@aopen_rec_term_core e2 0 (AE_FVar x)).
+   apply* (@aopent_atopent_rec_term_core t 0 (AT_TFVar x)).
+Proof.
+  induction 1; intros; simpl; f_equal*.
 Qed.
 
 Lemma atopen_rec_term : forall t u,
-  ATermTy t -> forall k, t = AOpenTypRec k u t.
+  ATerm t -> forall k, t = ATOpenRec k u t
+with atopent_rec_term : forall t u,
+  ATermTy t -> forall k, t = ATOpenTypRec k u t.
 Proof.
   induction 1; intros; simpl; f_equal*.
-  apply* aopen_rec_term.
-  unfolds AOpenT. pick_fresh x.
-   apply* (@atopen_rec_term_core t 0 (AE_FVar x)).
+  unfolds AOpen. pick_fresh x.
+   apply* (@atopen_aopen_rec_term_core e 0 (AE_FVar x)).
+  unfolds AOpen. pick_fresh x.
+   apply* (@atopent_aopent_rec_term_core t2 0 (AE_FVar x)).
+  unfolds AOpen. pick_fresh x.
+   apply* (@atopent_rec_term_core t 0 (AT_TFVar x)).
+Proof.
+  induction 1; intros; simpl; f_equal*.
 Qed.
 
-Lemma aopen_var_inj : forall x t1 t2, 
-  x \notin (AFv t1) -> x \notin (AFv t2) -> 
-  (t1 @ x = t2 @ x) -> (t1 = t2).
+Lemma aopen_var_inj : forall x t1 t2,
+  x \notin (AFv t1) -> x \notin (AFv t2) ->
+  forall k, (AOpenRec k (AE_FVar x) t1 = AOpenRec k (AE_FVar x) t2) -> (t1 = t2)
+with
+atopen_var_inj : forall x t1 t2,
+  x \notin (ATFv t1) -> x \notin (ATFv t2) ->
+  forall k, (AOpenTypRec k (AE_FVar x) t1 = AOpenTypRec k (AE_FVar x) t2) -> (t1 = t2).
 Proof.
-  intros x t1. unfold AOpen. generalize 0.
-  induction t1; intro k; destruct t2; simpl; intros; inversion H1;
-  try solve [ f_equal* 
-  | do 2 try case_nat; inversions* H1; try notin_false ].
+  intros x t1.
+  induction t1; intro t2.
+  destruct t2; simpl; intros;try(case_nat~). case_nat~. case_nat~.
+  inversion H1; subst. notin_false.
+  destruct t2; simpl; intros; try(case_nat~); try(solve[inversion H1]).
+  inversion H1; subst. notin_false.
+  inversion H1; subst~.
+  destruct t2; simpl; intros; try(case_nat~); try(solve[inversion H1]); auto.
+  destruct t2; simpl; intros; try(case_nat~); try(solve[inversion H1]); auto.
+  inversion H1; subst. f_equal ~. apply* IHt1_1. apply* IHt1_2.
+  destruct t2; simpl; intros; try(case_nat~); try(solve[inversion H1]); auto.
+  inversion H1; subst. f_equal ~. apply* IHt1.
+  destruct t2; simpl; intros; try(case_nat~); try(solve[inversion H1]); auto.
+  inversion H1; subst. f_equal ~. apply* atopen_var_inj. apply* atopen_var_inj.
+  destruct t2; simpl; intros; try(case_nat~); try(solve[inversion H1]); auto.
+  inversion H1; subst. f_equal ~. apply* IHt1.
+  destruct t2; simpl; intros; try(case_nat~); try(solve[inversion H1]); auto.
+  inversion H1; subst. f_equal ~. apply* IHt1.
+  destruct t2; simpl; intros; try(case_nat~); try(solve[inversion H1]); auto.
+  inversion H1; subst. f_equal ~. apply* IHt1. apply* atopen_var_inj.
+  destruct t2; simpl; intros; try(case_nat~); try(solve[inversion H1]); auto.
+  inversion H1; subst. f_equal ~. apply* atopen_var_inj.
+
+  intros x t1.
+  destruct t1; intros t2; destruct t2; simpl; intros; inversion H1; auto.
+  lets: aopen_var_inj H3; auto.
+  subst~.
 Qed.
 
 Lemma open_reorder: forall e1 e2 i j e,
     ATerm e1 ->
     ATerm e2 ->
     i <> j ->
-    AOpenRec i e1 (AOpenRec j e2 e) = AOpenRec j e2 (AOpenRec i e1 e).
-Proof.
-  introv te1 te2 neq.
-  gen i j. induction e; introv neq; simpls; auto; try(solve[f_equal ~]).
-  case_nat~. case_nat~. simpls. case_if~. symmetry. apply~ aopen_rec_term.
-  case_nat~. simpls. case_if~. apply~ aopen_rec_term.
-  simpls. case_if~. case_if~.
-Qed.
-
-Lemma notin_open_inv : forall x y n e,
-    x \notin AFv e ->
-    x \notin AFv y ->
-    x \notin AFv (AOpenRec n y e).
-Proof.
-  introv notin neq.
-  gen n. induction e; introv; simpls; auto.
-  case_if. auto. simpl.  auto.
-Qed.
-
-
-Lemma opent_reorder: forall e1 e2 i j e,
+    AOpenRec i e1 (AOpenRec j e2 e) = AOpenRec j e2 (AOpenRec i e1 e)
+with
+ opent_reorder: forall e1 e2 i j e,
     ATerm e1 ->
     ATerm e2 ->
     i <> j ->
@@ -116,62 +173,212 @@ Lemma opent_reorder: forall e1 e2 i j e,
 Proof.
   introv te1 te2 neq.
   gen i j. induction e; introv neq; simpls; auto; try(solve[f_equal ~]).
-  f_equal. apply~ open_reorder.
+  case_nat~. case_nat~. simpls. case_if~. symmetry. apply~ aopen_rec_term.
+  case_nat~. simpls. case_if~. apply~ aopen_rec_term.
+  simpls. case_if~. case_if~.
+Proof.
+  introv te1 te2 neq.
+  gen i j. induction e; introv neq; simpls; auto; try(solve[f_equal ~]).
 Qed.
 
-Lemma notin_opent_inv : forall x y n e,
+Lemma topen_reorder: forall e1 e2 i j e,
+    ATermTy e1 ->
+    ATermTy e2 ->
+    i <> j ->
+    ATOpenRec i e1 (ATOpenRec j e2 e) = ATOpenRec j e2 (ATOpenRec i e1 e)
+with
+topent_reorder: forall e1 e2 i j e,
+    ATermTy e1 ->
+    ATermTy e2 ->
+    i <> j ->
+    ATOpenTypRec i e1 (ATOpenTypRec j e2 e) = ATOpenTypRec j e2 (ATOpenTypRec i e1 e).
+Proof.
+  introv te1 te2 neq.
+  gen i j. induction e; introv neq; simpls; auto; try(solve[f_equal ~]).
+Proof.
+  introv te1 te2 neq.
+  gen i j. induction e; introv neq; simpls; auto; try(solve[f_equal ~]).
+  case_nat~. case_nat~. simpls. case_if~. symmetry. apply~ atopent_rec_term.
+  case_nat~. simpls. case_if~. apply~ atopent_rec_term.
+  simpls. case_if~. case_if~.
+Qed.
+
+Lemma notin_open_inv : forall x y n e,
+    x \notin AFv e ->
+    x \notin AFv y ->
+    x \notin AFv (AOpenRec n y e)
+with notin_opent_inv : forall x y n e,
     x \notin ATFv e ->
     x \notin AFv y ->
     x \notin ATFv (AOpenTypRec n y e).
 Proof.
   introv notin neq.
   gen n. induction e; introv; simpls; auto.
-  apply~ notin_open_inv.
+  case_if. auto. simpl.  auto.
+Proof.
+  introv notin neq.
+  gen n. induction e; introv; simpls; auto.
+Qed.
+
+Lemma notin_topen_inv : forall x y n e,
+    x \notin AFv e ->
+    x \notin ATFv y ->
+    x \notin AFv (ATOpenRec n y e)
+with notin_topent_inv : forall x y n e,
+    x \notin ATFv e ->
+    x \notin ATFv y ->
+    x \notin ATFv (ATOpenTypRec n y e).
+Proof.
+  introv notin neq.
+  gen n. induction e; introv; simpls; auto.
+Proof.
+  introv notin neq.
+  gen n. induction e; introv; simpls; auto.
+  case_if. auto. simpl.  auto.
 Qed.
 
 (* Substitution for a fresh name is identity. *)
 
 Lemma asubst_fresh : forall x t u, 
-  x \notin AFv t -> ASubst x u t = t.
-Proof.
-  intros. induction t; simpls; fequals*.
-  case_var*.
-  case_var*.
-Qed.
-
-Lemma atsubst_fresh : forall x t u, 
+  x \notin AFv t -> ASubst x u t = t
+with atsubst_fresh : forall x t u,
   x \notin ATFv t -> ATSubst x u t = t.
 Proof.
   intros. induction t; simpls; fequals*.
-  apply* asubst_fresh.
+  case_var*.
+Proof.
+  intros. induction t; simpls; fequals*.
 Qed.
 
-(* Substitution aistributes on the open operation. *)
+Lemma asubstt_fresh : forall x t u,
+  x \notin AFv t -> ASubstT x u t = t
+with atsubstt_fresh : forall x t u,
+  x \notin ATFv t -> ATSubstT x u t = t.
+Proof.
+  intros. induction t; simpls; fequals*.
+Proof.
+  intros. induction t; simpls; fequals*.
+  case_var*. case_var*.
+Qed.
+
+(* Substitution distributes on the open operation. *)
 
 Lemma asubst_openrec : forall n x u t1 t2, ATerm u -> 
-  ASubst x u (AOpenRec n t2 t1) = AOpenRec n (ASubst x u t2) (ASubst x u t1).
+  ASubst x u (AOpenRec n t2 t1) = AOpenRec n (ASubst x u t2) (ASubst x u t1)
+with
+atsubst_opentyprec : forall n x u t1 t2, ATerm u ->
+  ATSubst x u (AOpenTypRec n t2 t1) = AOpenTypRec n (ASubst x u t2) (ATSubst x u t1).
 Proof.
   intros. gen n.
   induction t1; intros; simpl; f_equal*.
   case_nat*. case_var*. apply* aopen_rec_term.
-  case_var*. apply* aopen_rec_term.
+Proof.
+  intros. induction t1; simpls; fequal *.
+Qed.
+
+Lemma asubst_topenrec : forall n x u t1 t2, ATerm u ->
+  ASubst x u (ATOpenRec n t2 t1) = ATOpenRec n (ATSubst x u t2) (ASubst x u t1)
+with
+atsubst_topentyprec : forall n x u t1 t2, ATerm u ->
+  ATSubst x u (ATOpenTypRec n t2 t1) = ATOpenTypRec n (ATSubst x u t2) (ATSubst x u t1).
+Proof.
+  intros. gen n.
+  induction t1; intros; simpl; f_equal*.
+  case_if*. apply* atopen_rec_term.
+Proof.
+  intros. induction t1; simpls; fequal *.
+  case_nat*.
+Qed.
+
+Lemma asubstt_openrec : forall n x u t1 t2, ATermTy u ->
+  ASubstT x u (AOpenRec n t2 t1) = AOpenRec n (ASubstT x u t2) (ASubstT x u t1)
+with
+atsubstt_opentyprec : forall n x u t1 t2, ATermTy u ->
+  ATSubstT x u (AOpenTypRec n t2 t1) = AOpenTypRec n (ASubstT x u t2) (ATSubstT x u t1).
+Proof.
+  intros. gen n.
+  induction t1; intros; simpl; f_equal*.
+  case_nat*.
+Proof.
+  intros. induction t1; simpls; fequal *.
+  case_if*. apply* aopent_rec_term.
+  case_if*. apply* aopent_rec_term.
+Qed.
+
+Lemma asubstt_topenrec : forall n x u t1 t2, ATermTy u ->
+  ASubstT x u (ATOpenRec n t2 t1) = ATOpenRec n (ATSubstT x u t2) (ASubstT x u t1)
+with
+atsubstt_topentyprec : forall n x u t1 t2, ATermTy u ->
+  ATSubstT x u (ATOpenTypRec n t2 t1) = ATOpenTypRec n (ATSubstT x u t2) (ATSubstT x u t1).
+Proof.
+  intros. gen n.
+  induction t1; intros; simpl; f_equal*.
+Proof.
+  intros. induction t1; simpls; fequal *.
+  case_nat*.
+  case_if*. apply* atopent_rec_term.
+  case_if*. apply* atopent_rec_term.
 Qed.
 
 Lemma asubst_open : forall x u t1 t2, ATerm u -> 
-  ASubst x u (t1 @@ t2) = (ASubst x u t1) @@ (ASubst x u t2).
+  ASubst x u (t1 @@ t2) = (ASubst x u t1) @@ (ASubst x u t2)
+with
+  atsubst_open : forall x u t1 t2, ATerm u ->
+  ATSubst x u (t1 @@' t2) = (ATSubst x u t1) @@' (ASubst x u t2).
 Proof.
   intros. apply* asubst_openrec.
-Qed.
-
-Lemma atsubst_open : forall x u t1 t2, ATerm u -> 
-  ATSubst x u (t1 @@' t2) = (ATSubst x u t1) @@' (ASubst x u t2).
 Proof.
   intros. unfold AOpenT. generalize 0.
   induction t1; intros; simpl; f_equal*.
   apply* asubst_openrec.
 Qed.
 
-(* Substitution and open_var for aistinct names commute. *)
+Lemma asubst_topen : forall x u t1 t2, ATerm u ->
+  ASubst x u (t1 @@# t2) = (ASubst x u t1) @@# (ATSubst x u t2)
+with
+  atsubst_topen : forall x u t1 t2, ATerm u ->
+  ATSubst x u (t1 @@#' t2) = (ATSubst x u t1) @@#' (ATSubst x u t2).
+Proof.
+  intros. apply* asubst_topenrec.
+Proof.
+  intros. unfold AOpenT. generalize 0.
+  induction t1; intros; simpl; f_equal*.
+  apply* atsubst_topentyprec.
+  unfold ATOpenT. simpls. f_equal *.
+Qed.
+
+Lemma asubstt_open : forall x u t1 t2, ATermTy u ->
+  ASubstT x u (t1 @@ t2) = (ASubstT x u t1) @@ (ASubstT x u t2)
+with
+  atsubstt_open : forall x u t1 t2, ATermTy u ->
+  ATSubstT x u (t1 @@' t2) = (ATSubstT x u t1) @@' (ASubstT x u t2).
+Proof.
+  intros. apply* asubstt_openrec.
+Proof.
+  intros. unfold AOpenT. generalize 0.
+  induction t1; intros; simpl; f_equal*.
+  case_if*. apply* aopent_rec_term.
+  case_if*. apply* aopent_rec_term.
+  apply* asubstt_openrec.
+Qed.
+
+Lemma asubstt_topen : forall x u t1 t2, ATermTy u ->
+  ASubstT x u (t1 @@# t2) = (ASubstT x u t1) @@# (ATSubstT x u t2)
+with
+  atsubstt_topen : forall x u t1 t2, ATermTy u ->
+  ATSubstT x u (t1 @@#' t2) = (ATSubstT x u t1) @@#' (ATSubstT x u t2).
+Proof.
+  intros. apply* asubstt_topenrec.
+Proof.
+  intros. unfold AOpenT. generalize 0.
+  induction t1; intros; simpl; f_equal*.
+  apply* atsubstt_topentyprec.
+  case_if*. apply* atopent_rec_term.
+  case_if*. apply* atopent_rec_term.
+  unfold ATOpenT. simpls. f_equal *.
+Qed.
+
+(* Substitution and open_var for distinct names commute. *)
 
 Lemma asubst_open_var : forall x y u e, y <> x -> ATerm u ->
   (ASubst x u e) @ y = ASubst x u (e @ y).
@@ -184,6 +391,44 @@ Lemma atsubst_open_var : forall x y u e, y <> x -> ATerm u ->
   (ATSubst x u e) @' y = ATSubst x u (e @' y).
 Proof.
   introv Neq Wu. rewrite* atsubst_open.
+  simpl. case_var*.
+Qed.
+
+Lemma asubst_open_tvar : forall x y u e, y <> x -> ATerm u ->
+  (ASubst x u e) @# y = ASubst x u (e @# y).
+Proof.
+  introv Neq Wu. rewrite* asubst_topen.
+Qed.
+
+Lemma atsubst_open_tvar : forall x y u e, y <> x -> ATerm u ->
+  (ATSubst x u e) @#' y = ATSubst x u (e @#' y).
+Proof.
+  introv Neq Wu. rewrite* atsubst_topen.
+Qed.
+
+Lemma asubstt_open_var : forall x y u e, y <> x -> ATermTy u ->
+  (ASubstT x u e) @ y = ASubstT x u (e @ y).
+Proof.
+  introv Neq Wu. rewrite* asubstt_open.
+Qed.
+
+Lemma atsubstt_open_var : forall x y u e, y <> x -> ATermTy u ->
+  (ATSubstT x u e) @' y = ATSubstT x u (e @' y).
+Proof.
+  introv Neq Wu. rewrite* atsubstt_open.
+Qed.
+
+Lemma asubstt_open_tvar : forall x y u e, y <> x -> ATermTy u ->
+  (ASubstT x u e) @# y = ASubstT x u (e @# y).
+Proof.
+  introv Neq Wu. rewrite* asubstt_topen.
+  simpl. case_var*.
+Qed.
+
+Lemma atsubstt_open_tvar : forall x y u e, y <> x -> ATermTy u ->
+  (ATSubstT x u e) @#' y = ATSubstT x u (e @#' y).
+Proof.
+  introv Neq Wu. rewrite* atsubstt_topen.
   simpl. case_var*.
 Qed.
 
@@ -206,6 +451,22 @@ Proof.
   rewrite* atsubst_fresh. simpl. case_var*.
 Qed.
 
+Lemma asubstt_intro : forall x t u,
+  x \notin (AFv t) -> ATermTy u ->
+  t @@# u = ASubstT x u (t @# x).
+Proof.
+  introv Fr Wu. rewrite* asubstt_topen.
+  rewrite* asubstt_fresh. simpl. case_var*.
+Qed.
+
+Lemma atsubstt_intro : forall x t u,
+  x \notin (ATFv t) -> ATermTy u ->
+  t @@#' u = ATSubstT x u (t @#' x).
+Proof.
+  introv Fr Wu. rewrite* atsubstt_topen.
+  rewrite* atsubstt_fresh. simpl. case_var*.
+Qed.
+
 (* Tactic to permute subst and open var *)
 
 Ltac cross := 
@@ -225,22 +486,37 @@ Tactic Notation "crosst" "*" :=
 (* Terms are stable by substitution *)
 
 Lemma asubst_term : forall t z u,
-  ATerm u -> ATerm t -> ATerm (ASubst z u t).
+  ATerm u -> ATerm t -> ATerm (ASubst z u t)
+with
+atsubst_term : forall t z u,
+  ATerm u -> ATermTy t -> ATermTy (ATSubst z u t)
+with
+asubstt_term : forall t z u,
+  ATermTy u -> ATerm t -> ATerm (ASubstT z u t)
+with
+atsubstt_term : forall t z u,
+  ATermTy u -> ATermTy t -> ATermTy (ATSubstT z u t).
 Proof.
   induction 2; simple*.
-  case_var*.
   case_var*.
   apply_fresh* ATerm_Lam as y. rewrite* asubst_open_var.
-  apply_fresh* ATerm_Pi as y. rewrite* asubst_open_var.
-  apply_fresh* ATerm_Let as y. rewrite* asubst_open_var.
-Qed.
-
-Lemma atsubst_term : forall t z u,
-  ATerm u -> ATermTy t -> ATermTy (ATSubst z u t).
+  apply_fresh* ATerm_Pi as y. rewrite* atsubst_open_var.
+  apply_fresh* ATerm_Forall as y. rewrite* atsubst_open_tvar.
 Proof.
   induction 2; simple*.
-  apply* ATermTy_Expr. apply* asubst_term.
-  apply_fresh* ATermTy_Forall as y. rewrite* atsubst_open_var.
+  apply~ ATermTy_TFVar.
+  apply~ ATermTy_EVar.
+  apply* ATermTy_Expr.
+Proof.
+  induction 2; simple*.
+  apply_fresh* ATerm_Lam as y. rewrite* asubstt_open_var.
+  apply_fresh* ATerm_Pi as y. rewrite* atsubstt_open_var.
+  apply_fresh* ATerm_Forall as y. rewrite* atsubstt_open_tvar.
+Proof.
+  induction 2; simple*.
+  case_var*. apply~ ATermTy_TFVar.
+  case_var*. apply~ ATermTy_EVar.
+  apply* ATermTy_Expr.
 Qed.
 
 (* Terms are stable by open *)
@@ -270,33 +546,15 @@ Proof.
 Qed.
 
 Lemma abody_pi : forall t1 t2,
-  ATerm (AE_Pi t1 t2) -> ABody t2.
+  ATerm (AE_Pi t1 t2) -> ABodyTy t2.
 Proof.
-  intros. unfold ABody. inversion* H.
-Qed.
-
-Lemma abody_let : forall e1 e2,
-  ATerm (AE_Let e1 e2) -> ABody e2.
-Proof.
-  intros. unfold ABody. inversion* H.
+  intros. unfold ABodyTy. inversion* H.
 Qed.
 
 Lemma aterm_pi : forall t1 t2,
-  ATerm (AE_Pi t1 t2) -> ATerm t1.
+  ATerm (AE_Pi t1 t2) -> ATermTy t1.
 Proof.
   intros. inversion* H.
-Qed.
-
-Lemma aterm_let : forall e1 e2,
-  ATerm (AE_Let e1 e2) -> ATerm e1.
-Proof.
-  intros. inversion* H.
-Qed.
-
-Lemma atermty_forall : forall e,
-  ATermTy (AT_Forall e) -> ABodyTy e.
-Proof.
-  intros. unfold ABodyTy. inversions* H.
 Qed.
 
 Lemma atermty_expr : forall e,
@@ -308,15 +566,12 @@ Qed.
 Hint Extern 1 (ATerm ?t) =>
   match goal with
   | H: ATerm (AE_Pi t ?t2) |- _ => apply (@aterm_pi t2)
-  | H: ATerm (AE_Let t ?t2) |- _ => apply (@aterm_let t2)
   | H: ATerm (AT_Expr ?t2) |- _ => apply (@atermty_expr t2)
   end.
 
 Hint Extern 3 (ABody ?t) =>
   match goal with 
   | H: context [AE_Lam t] |- _ => apply (@abody_lam)
-  | H: context [AE_Pi ?t1 t] |- _ => apply (@abody_pi t1)
-  | H: context [AE_Let ?t1 t] |- _ => apply (@abody_let t1)
   end.
 
 Hint Extern 1 (ABody ?t) =>
@@ -331,7 +586,7 @@ Hint Extern 1 (ABody ?t) =>
 
 Hint Extern 3 (ABodyTy ?t) =>
   match goal with 
-  | H: context [AT_Forall t] |- _ => apply (@atermty_forall)
+  | H: context [AE_Pi ?t1 t] |- _ => apply (@abody_pi t1)
   end.
 
 Hint Extern 1 (ABodyTy ?t) =>
@@ -352,21 +607,18 @@ Proof.
 Qed.
 
 Lemma aterm_pi_prove : forall t1 t2,
-  ATerm t1 -> ABody t2 -> ATerm (AE_Pi t1 t2).
+  ATermTy t1 -> ABodyTy t2 -> ATerm (AE_Pi t1 t2).
 Proof.
   intros. apply_fresh* ATerm_Pi as x.
 Qed.
 
-Lemma aterm_let_prove : forall e1 e2,
-  ATerm e1 -> ABody e2 -> ATerm (AE_Let e1 e2).
-Proof.
-  intros. apply_fresh* ATerm_Let as x.
-Qed.
-
 Lemma atermty_forall_prove : forall s,
-  ABodyTy s -> ATermTy (AT_Forall s).
+  ATermTy s -> ATerm (AE_Forall s).
 Proof.
-  intros. apply_fresh* ATermTy_Forall as x.
+  intros. apply_fresh* ATerm_Forall as x.
+  inversion H. unfold ATOpenT. simpls. apply* ATermTy_TFVar.
+  unfold ATOpenT. simpls. apply* ATermTy_EVar.
+  unfold ATOpenT. simpls. apply* ATermTy_Expr. subst. rewrite <- atopen_rec_term; auto.
 Qed.
 
 Lemma atermty_expr_prove : forall e,
@@ -376,7 +628,7 @@ Proof.
 Qed.
 
 Hint Resolve aterm_lam_prove
-     aterm_pi_prove aterm_let_prove
+     aterm_pi_prove
      atermty_forall_prove atermty_expr_prove.
 
 Lemma abody_prove : forall L t,
@@ -426,8 +678,6 @@ Hint Resolve abodyty_subst.
 Lemma ared_regular : forall t t', ARed t t' -> ATerm t /\ ATerm t'.
 Proof.
   intros_all. induction* H.
-  split*. apply* aopen_term.
-  apply* aterm_let.
 Qed.
 
 Hint Extern 1 (ATerm ?t) => match goal with
@@ -443,17 +693,11 @@ Hint Extern 1 (ATerm (AE_Pi (ASubst ?x ?u ?t1) (ASubst ?x ?u ?t2))) =>
   match goal with H: ATerm (AE_Pi t1 t2) |- _ => 
   unsimpl (ASubst x u (AE_Pi t1 t2)) end.
 
-Hint Extern 1 (ATerm (AE_Let (ASubst ?x ?u ?t1) (ASubst ?x ?u ?t2))) =>
-  match goal with H: ATerm (AE_Let t1 t2) |- _ => 
-  unsimpl (ASubst x u (AE_Let t1 t2)) end.
-
-Hint Extern 1 (ATermTy (AT_Forall (ATSubst ?x ?u ?t2))) =>
-  match goal with H: ATermTy (AT_Forall t2) |- _ => 
-  unsimpl (ATSubst x u (AT_Forall t2)) end.
+Hint Extern 1 (ATerm (AE_Forall ?v (ATSubst ?x ?u ?t2))) =>
+  match goal with H: ATerm (AE_Forall v t2) |- _ =>
+  unsimpl (ATSubst x u (AE_Forall t2)) end.
 
 Definition regular_actx (E : ACtx) :=
   AWf E /\ ok E /\
-  (forall x U, binds x (AC_Typ U) E -> ATerm U) /\
-  (forall x T U, binds x (AC_Bnd T U) E -> ATermTy T /\ ATerm U) /\
-  (forall x T, binds x (AC_Solved_EVar T) E -> ATerm T).
-
+  (forall x U, binds x (AC_Typ U) E -> ATermTy U) /\
+  (forall x T, binds x (AC_Solved_EVar T) E -> ATermTy T).
